ProximityPrize/SubmissionLower/LocatorSourceArithmetic.lean
@@ -2,7 +2,7 @@ import ProximityPrize.SubmissionLower.LocatorArithmetic
 namespace ProximityPrize.SubmissionLower.LocatorSourceArithmetic
 open RCN100 RCN119 RCN302
 theorem kernelAmbient_nullity:
-    coefficientCount 22896342 131071 52091 39 -
-      262144 * localRankBound 126 52091 39=18421074905050:=
+    coefficientCount 27253050 131071 36564 45 -
+      262144 * localRankBound 150 36564 45=21870099643880:=
   LocatorArithmetic.kernelC_nullity
 end ProximityPrize.SubmissionLower.LocatorSourceArithmetic
